feat: functional induction for structural recursion (#3738)
This extends `derive_functional_induction` to work with structural
recursion as well.

It produces the less general, more concrete induction rule where the
induction hypothesis is
specialized for every argument of the recursive call, not just the the
one that the function
is recursing on.

Care is taken so that the induction principle and it's motive take the
arguments in the same
order as the original function.

While I was it, also makes sure that the order of the cases in the
induction principle matches
the order of recursive calls in the function better.

---------

Co-authored-by: David Thrane Christiansen <david@davidchristiansen.dk>
Co-authored-by: Leonardo de Moura <leomoura@amazon.com>

tests/lean/run/funind_fewer_levels.lean
@@ -4,6 +4,26 @@ This test checks if the functional induction principle has fewer universe parame
 if the original function has a parameter that disappears.
 -/
 
+namespace Structural
+def foo.{u} : Nat → PUnit.{u}
+| 0 => .unit
+| n+1 => foo n
+
+derive_functional_induction foo
+/--
+info: Structural.foo.induct (motive : Nat → Prop) (case1 : motive 0) (case2 : ∀ (n : Nat), motive n → motive n.succ) :
+  ∀ (a : Nat), motive a
+-/
+#guard_msgs in
+#check foo.induct
+
+example : foo n = .unit := by
+  induction n using foo.induct with
+  | case1 => unfold foo; rfl
+  | case2 n ih => unfold foo; exact ih
+
+end Structural
+
 namespace WellFounded
 def foo.{u,v} {α : Type v} : List α  → PUnit.{u}
 | [] => .unit
@@ -13,7 +33,7 @@ termination_by xs => xs
 derive_functional_induction foo
 /--
 info: WellFounded.foo.induct.{v} {α : Type v} (motive : List α → Prop) (case1 : motive [])
-  (case2 : ∀ (head : α) (xs : List α), motive xs → motive (head :: xs)) (x : List α) : motive x
+  (case2 : ∀ (head : α) (xs : List α), motive xs → motive (head :: xs)) : ∀ (a : List α), motive a
 -/
 #guard_msgs in
 #check foo.induct
