tests/lean/run/funind_tests.lean
@@ -11,8 +11,8 @@ derive_functional_induction ackermann
 /--
 info: Unary.ackermann.induct (motive : Nat × Nat → Prop) (case1 : ∀ (m : Nat), motive (0, m))
   (case2 : ∀ (n : Nat), motive (n, 1) → motive (n.succ, 0))
-  (case3 : ∀ (n m : Nat), motive (n + 1, m) → motive (n, ackermann (n + 1, m)) → motive (n.succ, m.succ))
-  (x : Nat × Nat) : motive x
+  (case3 : ∀ (n m : Nat), motive (n + 1, m) → motive (n, ackermann (n + 1, m)) → motive (n.succ, m.succ)) :
+  ∀ (a : Nat × Nat), motive a
 -/
 #guard_msgs in
 #check ackermann.induct
@@ -49,7 +49,7 @@ derive_functional_induction Tree.rev
 
 /--
 info: Tree.rev.induct (motive : Tree → Prop)
-  (case1 : ∀ (ts : List Tree), (∀ (t : Tree), t ∈ ts → motive t) → motive (Tree.node ts)) (x : Tree) : motive x
+  (case1 : ∀ (ts : List Tree), (∀ (t : Tree), t ∈ ts → motive t) → motive (Tree.node ts)) : ∀ (a : Tree), motive a
 -/
 #guard_msgs in
 #check Tree.rev.induct
@@ -64,7 +64,7 @@ termination_by n => n
 derive_functional_induction fib
 /--
 info: fib.induct (motive : Nat → Prop) (case1 : motive 0) (case2 : motive 1)
-  (case3 : ∀ (n : Nat), motive n → motive (n + 1) → motive n.succ.succ) (x : Nat) : motive x
+  (case3 : ∀ (n : Nat), motive n → motive (n + 1) → motive n.succ.succ) : ∀ (a : Nat), motive a
 -/
 #guard_msgs in
 #check fib.induct
@@ -79,8 +79,8 @@ termination_by n => n
 derive_functional_induction have_tailrec
 
 /--
-info: have_tailrec.induct (motive : Nat → Prop) (case1 : motive 0) (case2 : ∀ (n : Nat), n < n + 1 → motive n → motive n.succ)
-  (x : Nat) : motive x
+info: have_tailrec.induct (motive : Nat → Prop) (case1 : motive 0)
+  (case2 : ∀ (n : Nat), n < n + 1 → motive n → motive n.succ) : ∀ (a : Nat), motive a
 -/
 #guard_msgs in
 #check have_tailrec.induct
@@ -96,8 +96,8 @@ termination_by n => n
 derive_functional_induction have_non_tailrec
 
 /--
-info: have_non_tailrec.induct (motive : Nat → Prop) (case1 : motive 0) (case2 : ∀ (n : Nat), motive n → motive n.succ)
-  (x : Nat) : motive x
+info: have_non_tailrec.induct (motive : Nat → Prop) (case1 : motive 0) (case2 : ∀ (n : Nat), motive n → motive n.succ) :
+  ∀ (a : Nat), motive a
 -/
 #guard_msgs in
 #check have_non_tailrec.induct
@@ -116,8 +116,8 @@ info: let_tailrec.induct (motive : Nat → Prop) (case1 : motive 0)
   (case2 :
     ∀ (n : Nat),
       let h2 := ⋯;
-      motive n → motive n.succ)
-  (x : Nat) : motive x
+      motive n → motive n.succ) :
+  ∀ (a : Nat), motive a
 -/
 #guard_msgs in
 #check let_tailrec.induct
@@ -133,8 +133,8 @@ termination_by n => n
 derive_functional_induction let_non_tailrec
 
 /--
-info: let_non_tailrec.induct (motive : Nat → Prop) (case1 : motive 0) (case2 : ∀ (n : Nat), motive n → motive n.succ)
-  (x : Nat) : motive x
+info: let_non_tailrec.induct (motive : Nat → Prop) (case1 : motive 0) (case2 : ∀ (n : Nat), motive n → motive n.succ) :
+  ∀ (a : Nat), motive a
 -/
 #guard_msgs in
 #check let_non_tailrec.induct
@@ -154,7 +154,7 @@ derive_functional_induction with_ite_tailrec
 /--
 info: with_ite_tailrec.induct (motive : Nat → Prop) (case1 : motive 0)
   (case2 : ∀ (n : Nat), n % 2 = 0 → motive n → motive n.succ)
-  (case3 : ∀ (n : Nat), ¬n % 2 = 0 → motive n → motive n.succ) (x : Nat) : motive x
+  (case3 : ∀ (n : Nat), ¬n % 2 = 0 → motive n → motive n.succ) : ∀ (a : Nat), motive a
 -/
 #guard_msgs in
 #check with_ite_tailrec.induct
@@ -175,7 +175,7 @@ derive_functional_induction with_ite_non_tailrec
 
 /--
 info: with_ite_non_tailrec.induct (motive : Nat → Prop) (case1 : motive 0) (case2 : motive 1)
-  (case3 : ∀ (n : Nat), motive (n + 1) → motive n → motive n.succ.succ) (x : Nat) : motive x
+  (case3 : ∀ (n : Nat), motive (n + 1) → motive n → motive n.succ.succ) : ∀ (a : Nat), motive a
 -/
 #guard_msgs in
 #check with_ite_non_tailrec.induct
@@ -191,9 +191,8 @@ termination_by n
 derive_functional_induction with_dite_non_tailrec
 
 /--
-info: with_dite_non_tailrec.induct (motive : Nat → Prop)
-(case1 : ∀ (x : Nat), (x - 1 < x → motive (x - 1)) → motive x)
-  (x : Nat) : motive x
+info: with_dite_non_tailrec.induct (motive : Nat → Prop) (case1 : ∀ (x : Nat), (x - 1 < x → motive (x - 1)) → motive x)
+  (n : Nat) : motive n
 -/
 #guard_msgs in
 #check with_dite_non_tailrec.induct
@@ -208,9 +207,8 @@ termination_by n
 derive_functional_induction with_dite_tailrec
 
 /--
-info: with_dite_tailrec.induct (motive : Nat → Prop)
-(case1 : ∀ (x : Nat), x - 1 < x → motive (x - 1) → motive x)
-  (case2 : ∀ (x : Nat), ¬x - 1 < x → motive x) (x : Nat) : motive x
+info: with_dite_tailrec.induct (motive : Nat → Prop) (case1 : ∀ (x : Nat), x - 1 < x → motive (x - 1) → motive x)
+  (case2 : ∀ (x : Nat), ¬x - 1 < x → motive x) (n : Nat) : motive n
 -/
 #guard_msgs in
 #check with_dite_tailrec.induct
@@ -227,7 +225,7 @@ derive_functional_induction with_match_refining_tailrec
 
 /--
 info: with_match_refining_tailrec.induct (motive : Nat → Prop) (case1 : motive 0) (case2 : motive 0 → motive (Nat.succ 0))
-  (case3 : ∀ (m : Nat), (m = 0 → False) → motive m → motive m.succ) (x : Nat) : motive x
+  (case3 : ∀ (m : Nat), (m = 0 → False) → motive m → motive m.succ) : ∀ (a : Nat), motive a
 -/
 #guard_msgs in
 #check with_match_refining_tailrec.induct
@@ -278,7 +276,7 @@ derive_functional_induction with_other_match_tailrec
 /--
 info: with_other_match_tailrec.induct (motive : Nat → Prop) (case1 : motive 0)
   (case2 : ∀ (n : Nat), n % 2 = 0 → motive n → motive n.succ)
-  (case3 : ∀ (n : Nat), (n % 2 = 0 → False) → motive n → motive n.succ) (x : Nat) : motive x
+  (case3 : ∀ (n : Nat), (n % 2 = 0 → False) → motive n → motive n.succ) : ∀ (a : Nat), motive a
 -/
 #guard_msgs in
 #check with_other_match_tailrec.induct
@@ -331,8 +329,8 @@ termination_by n => n
 derive_functional_induction with_match_non_tailrec
 
 /--
-info: with_match_non_tailrec.induct (motive : Nat → Prop) (case1 : motive 0) (case2 : ∀ (n : Nat), motive n → motive n.succ)
-  (x : Nat) : motive x
+info: with_match_non_tailrec.induct (motive : Nat → Prop) (case1 : motive 0) (case2 : ∀ (n : Nat), motive n → motive n.succ) :
+  ∀ (a : Nat), motive a
 -/
 #guard_msgs in
 #check with_match_non_tailrec.induct
@@ -355,8 +353,8 @@ info: with_match_non_tailrec_refining.induct (motive : Nat → Prop) (case1 : mo
       (match n with
         | 0 => motive 0
         | m => motive m) →
-        motive n.succ)
-  (x : Nat) : motive x
+        motive n.succ) :
+  ∀ (a : Nat), motive a
 -/
 #guard_msgs in
 #check with_match_non_tailrec_refining.induct
@@ -373,8 +371,8 @@ derive_functional_induction with_overlap
 
 /--
 info: with_overlap.induct (motive : Nat → Prop) (case1 : motive 0) (case2 : motive 1) (case3 : motive 2) (case4 : motive 3)
-  (case5 : ∀ (n : Nat), (n = 0 → False) → (n = 1 → False) → (n = 2 → False) → motive n → motive n.succ) (x : Nat) :
-  motive x
+  (case5 : ∀ (n : Nat), (n = 0 → False) → (n = 1 → False) → (n = 2 → False) → motive n → motive n.succ) :
+  ∀ (a : Nat), motive a
 -/
 #guard_msgs in
 #check with_overlap.induct
@@ -392,7 +390,7 @@ derive_functional_induction unary
 
 /--
 info: UnusedExtraParams.unary.induct (base : Nat) (motive : Nat → Prop) (case1 : motive 0)
-  (case2 : ∀ (n : Nat), motive n → motive n.succ) (x : Nat) : motive x
+  (case2 : ∀ (n : Nat), motive n → motive n.succ) : ∀ (a : Nat), motive a
 -/
 #guard_msgs in
 #check unary.induct
@@ -443,7 +441,7 @@ info: NonTailrecMatch.match_non_tail.induct (motive : Nat → Prop)
         | 1 => True
         | n.succ.succ => motive n ∧ motive (n + 1)) →
         motive x)
-  (x : Nat) : motive x
+  (n : Nat) : motive n
 -/
 #guard_msgs in
 #check match_non_tail.induct
@@ -469,7 +467,7 @@ derive_functional_induction foo
 
 /--
 info: AsPattern.foo.induct (motive : Nat → Prop) (case1 : motive 0) (case2 : ∀ (n : Nat), motive n → motive n.succ)
-  (x : Nat) : motive x
+  (n : Nat) : motive n
 -/
 #guard_msgs in
 #check foo.induct
@@ -492,7 +490,7 @@ info: AsPattern.bar.induct (motive : Nat → Prop)
         | 0 => True
         | x@h:n.succ => motive n) →
         motive x)
-  (x : Nat) : motive x
+  (n : Nat) : motive n
 -/
 #guard_msgs in
 #check bar.induct
@@ -526,7 +524,7 @@ decreasing_by
 derive_functional_induction foo
 /--
 info: GramSchmidt.foo.induct (motive : Nat → Prop) (case1 : ∀ (x : Nat), (∀ (i : Nat), below x i → motive i) → motive x)
-  (x : Nat) : motive x
+  (n : Nat) : motive n
 -/
 #guard_msgs in
 #check foo.induct
@@ -544,7 +542,7 @@ termination_by xs => xs
 derive_functional_induction foo
 /--
 info: LetFun.foo.induct.{u_1} {α : Type u_1} (x : α) (motive : List α → Prop) (case1 : motive [])
-  (case2 : ∀ (_y : α) (ys : List α), motive ys → motive (_y :: ys)) : ∀ (x : List α), motive x
+  (case2 : ∀ (_y : α) (ys : List α), motive ys → motive (_y :: ys)) : ∀ (a : List α), motive a
 -/
 #guard_msgs in
 #check foo.induct
@@ -560,7 +558,7 @@ termination_by xs => xs
 derive_functional_induction bar
 /--
 info: LetFun.bar.induct.{u_1} {α : Type u_1} (x : α) (motive : List α → Prop) (case1 : motive [])
-  (case2 : ∀ (_y : α) (ys : List α), motive ys → motive (_y :: ys)) : ∀ (x : List α), motive x
+  (case2 : ∀ (_y : α) (ys : List α), motive ys → motive (_y :: ys)) : ∀ (a : List α), motive a
 -/
 #guard_msgs in
 #check bar.induct
@@ -579,12 +577,13 @@ derive_functional_induction foo
 /--
 info: RecCallInDisrs.foo.induct (motive : Nat → Prop) (case1 : motive 0)
   (case2 : ∀ (n : Nat), foo n = 0 → motive n → motive n.succ)
-  (case3 : ∀ (n : Nat), ¬foo n = 0 → motive n → motive n.succ) (x : Nat) : motive x
+  (case3 : ∀ (n : Nat), ¬foo n = 0 → motive n → motive n.succ) : ∀ (a : Nat), motive a
 -/
 #guard_msgs in
 #check foo.induct
 
 
+set_option linter.unusedVariables false in
 def bar : Nat → Nat
   | 0 => 0
   | n+1 => match _h : n, bar n with
@@ -597,7 +596,7 @@ derive_functional_induction bar
 /--
 info: RecCallInDisrs.bar.induct (motive : Nat → Prop) (case1 : motive 0) (case2 : bar 0 = 0 → motive 0 → motive (Nat.succ 0))
   (case3 : (bar 0 = 0 → False) → motive 0 → motive (Nat.succ 0))
-  (case4 : ∀ (m : Nat), motive m.succ → motive m → motive m.succ.succ) (x : Nat) : motive x
+  (case4 : ∀ (m : Nat), motive m.succ → motive m → motive m.succ.succ) : ∀ (a : Nat), motive a
 -/
 #guard_msgs in
 #check bar.induct
@@ -679,7 +678,7 @@ derive_functional_induction unary
 
 /--
 info: DefaultArgument.unary.induct (fixed : Bool) (motive : Nat → Prop) (case1 : motive 0)
-  (case2 : ∀ (n : Nat), motive n → motive n.succ) (x : Nat) : motive x
+  (case2 : ∀ (n : Nat), motive n → motive n.succ) (n : Nat) : motive n
 -/
 #guard_msgs in
 #check unary.induct
@@ -745,7 +744,7 @@ info: Dite.foo.induct (motive : Nat → Prop)
     ∀ (x : Nat),
       let j := x - 1;
       ¬j < x → motive x)
-  (x : Nat) : motive x
+  (n : Nat) : motive n
 -/
 #guard_msgs in
 #check foo.induct
@@ -824,11 +823,11 @@ where
   termination_by as.size - i
 
 /--
-error: Function Errors.takeWhile does not look like a function defined by well-founded recursion.
+error: Function Errors.takeWhile does not look like a function defined by recursion.
 NB: If Errors.takeWhile is not itself recursive, but contains an inner recursive function (via `let rec` or `where`), try `Errors.takeWhile.go` where `go` is name of the inner function.
 -/
 #guard_msgs in
-derive_functional_induction takeWhile -- Cryptic error message
+derive_functional_induction takeWhile
 
 derive_functional_induction takeWhile.foo
 
@@ -853,7 +852,7 @@ derive_functional_induction foo
 /--
 info: PreserveParams.foo.induct (a : Nat) (motive : Nat → Prop) (case1 : motive 0)
   (case2 : ∀ (n : Nat), a = 23 → motive n.succ) (case3 : ¬a = 23 → motive a.succ)
-  (case4 : ∀ (n : Nat), ¬a = 23 → ¬a = n → motive n → motive n.succ) (x : Nat) : motive x
+  (case4 : ∀ (n : Nat), ¬a = 23 → ¬a = n → motive n → motive n.succ) : ∀ (a : Nat), motive a
 -/
 #guard_msgs in
 #check foo.induct
